alloc_metadata 12/n: allocate_sizeclass WIP
lets check extraction

src/SizeClass2.fst
@@ -75,9 +75,6 @@ let size_class_vprop
     (vptr r)
     (fun scs -> size_class_vprop_aux scs)
 
-#restart-solver
-
-#push-options "--z3rlimit 20"
 let size_class_vprop_test
   (r: ref size_class_struct)
   : Steel unit
@@ -90,109 +87,58 @@ let size_class_vprop_test
     h1 (size_class_vprop r)
   )
   =
-  let x0 = gget (size_class_vprop r) in
   let x = elim_vdep (vptr r) (fun scs -> size_class_vprop_aux scs) in
   intro_vdep
     (vptr r)
     (size_class_vprop_aux (G.reveal x))
     (fun scs -> size_class_vprop_aux scs);
-  let x1 = gget (size_class_vprop r) in
-  assert (dfst x1 == dfst x0);
-  assert (dsnd x1 == dsnd x0)
-#pop-options
+  admit ()
 
-(*)
-let size_class_sl'
+
+#push-options "--z3rlimit 50"
+let allocate_size_class
   (r: ref size_class_struct)
-  (scs: size_class_struct)
-  : SM.slprop u#1
+  //: Steel unit
+  : Steel (array U8.t)
+  (size_class_vprop r)
+  (fun result ->
+    A.varray result `star`
+    size_class_vprop r)
+  (requires fun h0 -> True)
+  (ensures fun h0 _ h1 -> True)
   =
-  pts_to_sl r P.full_perm scs `SM.star`
-  SL.ind_llist_sl (p_partial scs.size) (scs.partial_slabs) `SM.star`
-  SL.ind_llist_sl (p_empty scs.size) (scs.empty_slabs) `SM.star`
-  vrefinedep_hp
-    (vptr scs.md_count)
-    //TODO: hideous coercion
-    (fun x -> U32.v x <= U32.v metadata_max == true)
-    (fun v ->
-      A.varray (A.split_r scs.slab_region (u32_to_sz (U32.mul v page_size))) `star`
-      A.varray (A.split_r scs.md_bm_region (u32_to_sz (U32.mul v 4ul))) `star`
-      A.varray (A.split_r scs.md_region (u32_to_sz v)))
-
-let size_class_sl
-  (r: ref size_class_struct)
-  : SM.slprop u#1
-  =
-  SM.h_exists (size_class_sl' r)
-
-
-let size_class_sl'_witinv (r: ref size_class_struct)
-  : Lemma (SM.is_witness_invariant (size_class_sl' r))
-  =
-  let aux (scs1 scs2: size_class_struct) (m: SM.mem)
-  : Lemma
-  (requires
-    SM.interp (size_class_sl' r scs1) m /\
-    SM.interp (size_class_sl' r scs2) m
-  )
-  (ensures scs1 == scs2)
-  =
-  pts_to_witinv r P.full_perm;
-  assert (scs1 == scs2)
-  in
-  Classical.forall_intro_3 (Classical.move_requires_3 aux)
-
-let size_class_sel_full'
-  (r: ref size_class_struct)
-  : selector' blob2 (size_class_sl r)
-  =
-  fun (h:_) ->
-    let scs : size_class_struct = G.reveal (SM.id_elim_exists (size_class_sl' r) h) in
-    assert (SM.interp (size_class_sl' r scs) h);
-    let p1 = pts_to_sl r P.full_perm scs in
-    let p2 = SL.ind_llist_sl (p_partial scs.size) scs.partial_slabs in
-    let p3 = SL.ind_llist_sl (p_empty scs.size) scs.empty_slabs in
-    let p4 = vrefinedep_hp
+  let scs' = elim_vdep
+    (vptr r)
+    (fun scs -> size_class_vprop_aux scs) in
+  let scs = read r in
+  change_slprop_rel
+    (size_class_vprop_aux (G.reveal scs'))
+    (size_class_vprop_aux scs)
+    (fun x y -> x == y)
+    (fun _ -> admit ());
+  change_slprop_rel
+    (size_class_vprop_aux scs)
+    (SL.ind_llist (p_partial scs.size) scs.partial_slabs `star`
+    SL.ind_llist (p_empty scs.size) scs.empty_slabs `star`
+    vrefinedep
       (vptr scs.md_count)
+      //TODO: hideous coercion
       (fun x -> U32.v x <= U32.v metadata_max == true)
       (fun v ->
         A.varray (A.split_r scs.slab_region (u32_to_sz (U32.mul v page_size))) `star`
         A.varray (A.split_r scs.md_bm_region (u32_to_sz (U32.mul v 4ul))) `star`
-        A.varray (A.split_r scs.md_region (u32_to_sz v))) in
-    let sl = p1 `SM.star` p2 `SM.star` p3 `SM.star` p4 in
-    assert (SM.interp sl h);
-    let partial_slabs_v = SL.ind_llist_sel (p_partial scs.size) scs.partial_slabs h in
-    let empty_slabs_v = SL.ind_llist_sel (p_empty scs.size) scs.empty_slabs h in
-    let x = vrefinedep_sel
-      (vptr scs.md_count)
-      (fun x -> U32.v x <= U32.v metadata_max == true)
-      (fun v ->
-        A.varray (A.split_r scs.slab_region (u32_to_sz (U32.mul v page_size))) `star`
-        A.varray (A.split_r scs.md_bm_region (u32_to_sz (U32.mul v 4ul))) `star`
-        A.varray (A.split_r scs.md_region (u32_to_sz v))) h in
-    let md_count_v = dfst x in
-    //let y  ->
-    //    A.varray (A.split_r scs.slab_region (u32_to_sz (U32.mul v page_size))) `star`
-    //    A.varray (A.split_r scs.md_bm_region (u32_to_sz (U32.mul v 4ul))) `star`
-    //    A.varray (A.split_r scs.md_region (u32_to_sz v))
-    //)
-    let y
-    : t_of (
-        A.varray (A.split_r scs.slab_region (u32_to_sz (U32.mul md_count_v page_size))) `star`
-        A.varray (A.split_r scs.md_bm_region (u32_to_sz (U32.mul md_count_v 4ul))) `star`
-        A.varray (A.split_r scs.md_region (u32_to_sz md_count_v)))
-    = dsnd x in
-    let slab_region_v : Seq.seq U8.t = normalize_term ((fun (a, _, _) -> a) y) in
-    let md_bm_region_v : Seq.seq U64.t = (fun (_, b, _) -> b) y in
-    let md_region_v : Seq.seq (SL.cell blob) = (fun (_, _, c) -> c) y in
-    //let (slab_region_v, md_bm_region_v, md_region_v) = y in
-    let b = {
-      scs_v = G.reveal scs;
-      partial_slabs_v = partial_slabs_v;
-      empty_slabs_v = empty_slabs_v;
-      md_count_v = md_count_v;
-      slab_region_v = slab_region_v;
-      md_bm_region_v = md_bm_region_v;
-      md_region_v = md_region_v;
-    } in
-    b
+        A.varray (A.split_r scs.md_region (u32_to_sz v))
+      )
+    )
+    (fun x y -> x == y)
+    (fun _ -> admit ());
+  let result = allocate_slab
+    scs.size scs.partial_slabs scs.empty_slabs
+    scs.slab_region scs.md_bm_region scs.md_region
+    scs.md_count in
+  sladmit ();
+  //intro_vdep
+  //  (vptr r)
+  //  (size_class_vprop_aux scs)
+  //  (fun scs -> size_class_vprop_aux scs);
+  return result
